fstar/new/Crypto.fsti
@@ -63,71 +63,18 @@ type sign_signature (cs:ciphersuite) = lbytes (sign_signature_length cs)
 val sign_sign: cs:ciphersuite -> sign_private_key cs -> bytes -> randomness (sign_nonce_length cs) -> result (sign_signature cs)
 val sign_verify: cs:ciphersuite -> sign_public_key cs -> bytes -> sign_signature cs -> bool
 
+(*** AEAD ***)
+
+val aead_nonce_length: ciphersuite -> size_nat
+val aead_key_length: ciphersuite -> size_nat
+
+type aead_key (cs:ciphersuite) = lbytes (aead_key_length cs)
+type aead_nonce (cs:ciphersuite) = lbytes (aead_nonce_length cs)
+
+val aead_encrypt: cs:ciphersuite -> aead_key cs -> aead_nonce cs -> ad:bytes -> plaintext:bytes -> result bytes
+val aead_decrypt: cs:ciphersuite -> aead_key cs -> aead_nonce cs -> ad:bytes -> ciphertext:bytes -> result bytes
+
 (*** String to bytes ***)
 
 let string_is_ascii (s:string) = List.Tot.for_all (fun x -> FStar.Char.int_of_char x < 256) (FStar.String.list_of_string s)
 val string_to_bytes: s:string{b2t (normalize_term (string_is_ascii s && String.strlen s < max_size_t))} -> lbytes (String.strlen s)
-
-(*
-open FStar.Mul
-open Lib.IntTypes
-open Lib.Sequence
-open Lib.ByteSequence
-open Lib.LoopCombinators
-open Lib.RandomSequence
-open Lib.Result
-
-#set-options "--z3rlimit 150"
-
-(** Definition of bytes *)
-(* val bytes : Type0 *)
-(* val length_of_bytes: bytes -> nat *)
-(* val eq_bytes: bytes -> bytes -> bool // use sparingly *)
-
-
-(** Definition of concrete bytes *)
-let bytes_t = Seq.seq nat
-let pub_bytes_t = Seq.seq nat
-
-(* Empty bytes *)
-let empty_bytes = Seq.empty
-
-(* Conversion from integers to public bytes *)
-val nat_to_bytes: nat -> bytes_t
-val nat_to_n_bytes: nat -> nat -> bytes_t
-val nat_of_bytes: bytes_t -> result nat
-
-(* Concatenation and split for public bytes *)
-val concat: bytes_t -> bytes_t -> bytes_t
-val split: bytes_t -> result (bytes_t & bytes_t)
-val split_lemma1: a:bytes_t -> b:bytes_t ->
-    Lemma (ensures (split (concat a b) == Success (a,b)))
-    [SMTPat (split (concat a b))]
-val split_lemma2: m:bytes_t ->
-    Lemma (match split m with
-           | Success (a,b) -> m == concat a b
-	   | _ -> True)
-    [SMTPat (split m)]
-
-val derive: bytes_t -> string -> bytes_t -> result bytes_t
-val derive_extract: bytes_t -> bytes_t -> result bytes_t
-val derive_expand_label: bytes_t -> string -> bytes_t -> nat -> result bytes_t
-
-val secret_to_public: bytes_t -> result pub_bytes_t
-val pke_enc: pub_bytes_t -> bytes_t -> result pub_bytes_t
-val pke_dec: bytes_t -> pub_bytes_t -> result bytes_t
-
-val sign: bytes_t -> bytes_t -> result bytes_t
-val verify: bytes_t -> bytes_t -> bytes_t -> bool
-
-val aead_enc: s:bytes_t -> b:bytes_t -> n:bytes_t -> ad:bytes_t -> result bytes_t
-val aead_dec: s:bytes_t -> enc:bytes_t -> n:bytes_t -> ad:bytes_t -> result bytes_t
-
-val pad: bytes_t -> nat -> result bytes_t
-val unpad: bytes_t -> result bytes_t
-
-val hash: bytes_t -> result bytes_t
-val mac: bytes_t -> bytes_t -> result bytes_t
-val mac_verify: bytes_t -> bytes_t -> bytes_t -> bool
-
-*)
